{
 "cells": [
  {
   "cell_type": "markdown",
   "metadata": {},
   "source": [
    "# Using the Laplace Transform to solve Differential Equations\n",
    "\n",
    "We now begin to apply the Laplace Transform to solving constant coefficient linear differential equations.  We focus on differential equations of the form\n",
    "\n",
    "$$f'(t) + af(t) = g(t)$$\n",
    "\n",
    "and\n",
    "\n",
    "$$f''(t) + af'(t) + bf(t) = g(t)$$\n",
    "\n",
    "The process will be to \n",
    "- Take the Laplace Transform of both sides of the differential equation (using the initial conditions)\n",
    "- Do some Algebra to solve for $\\tilde{f}(s)$.\n",
    "- Invert the Laplace Transform of $\\tilde{f}(s)$ to find $f(t)$.\n"
   ]
  },
  {
   "cell_type": "markdown",
   "metadata": {},
   "source": [
    "## Transforms of $f'(t)$ and $f''(t)$\n",
    "To take the Laplace Transform of our differential equations, we will need to know the transforms of $f'(t)$ and $f''(t)$.  \n",
    "\n",
    "\n",
    "````{prf:theorem} Transforms of derivatives\n",
    "\n",
    "Given a function $f(t)$ whose Laplace Transform is $\\tilde{f}(s)$, the transform of $f'(t)$ and $f''(t)$ are\n",
    "\\begin{align*}\n",
    "\\mathcal{L}[f'(t)](s) &= s\\tilde{f}(s) - f(0)\\\\\n",
    "\\mathcal{L}[f''(t)](s) &= s^2 \\tilde{f}(s) - sf(0) - f'(0)\n",
    "\\end{align*}\n",
    "````\n",
    "To demonstrate this for $f'(t)$, we turn to the definition of the Laplace Transform:\n",
    "\\begin{align*}\n",
    "\\mathcal{L}[f'(t)](s) &= \\int_0^\\infty f'(t) e^{-st} \\, dt\\\\\n",
    " &=  \\left. f(t)e^{-st} \\right|_0^\\infty - \\int_0^\\infty f(t)(-s)e^{-st} \\, dt\\\\\n",
    " &= 0 - f(0) + s \\int_0^\\infty f(t) e^{-st} \\, dt\\\\\n",
    " &= -f(0) + s \\tilde{f}(s)\n",
    " \\end{align*}\n",
    "A similar demonstration applies to $\\mathcal{L}[f''(t)](s)$. \n",
    "\n",
    "\n",
    "So the transforms of $f'(t)$ and $f''(t)$ can be written in terms of the transform of $f(t)$ and the initial conditions.  This is the key detail that leads to the Laplace Transform of a differential equation for $f(t)$ becoming an Algebraic equation for $\\tilde{f}(s)$.\n",
    "\n",
    "\n",
    "\n"
   ]
  },
  {
   "cell_type": "markdown",
   "metadata": {},
   "source": [
    "## Examples\n",
    "\n",
    "````{prf:example} $f''(t) + 4f'(t) + 3f(t) = -6e^{-3t}$\n",
    "\n",
    "To find $f(t)$ if $f''(t) + 4f'(t) + 3f(t) = -6e^{-3t}$ with $f(0) = 1$ and $f'(0)=-2$ we take the Transform of both sides:\n",
    "\\begin{align*}\n",
    "f''(t) + 4f'(t) + 3f(t) &= -6e^{-3t}\\\\\n",
    "\\Rightarrow \\quad \\mathcal{L}[f''(t) + 4f'(t) + 3f(t)](s) &= \\mathcal{L}\\left[-6e^{-3t}\\right](s)\\\\\n",
    "s^2\\tilde{f}(s) - sf(0) - f'(0) + 4(s\\tilde{f}(s) - f(0)) + 3 \\tilde{f}(s) &= \\frac{-6}{s+3}\\\\\n",
    "(s^2+4s+3)\\tilde{f}(s) - s + 2 -4 &= \\frac{-6}{s+3}\\\\\n",
    "\\tilde{f}(s) &= \\frac{-6}{(s+3)(s^2+4s+3)} + \\frac{s+2}{s^2+4s+3}\\\\\n",
    "&= \\frac{-6}{(s+3)^2(s+1)} + \\frac{s+2}{(s+3)(s+1)}\n",
    "\\end{align*}\n",
    "\n",
    "We have solved for $\\tilde{f}(s)$.  Now we just need to invert the transform.  We could approach each fraction separately or we could do a single partial fractions expansion.  Typically if you can't tell immediately how one of the fractions would be rewritten, it is easiest to do them in a single expansion.  The common denominator is $(s+3)^2(s+1)$.  So we have\n",
    "\n",
    "$$\n",
    "\\frac{-6 + (s+2)(s+3)}{(s+3)^2(s+1)} = \\frac{A}{(s+3)^2} + \\frac{B}{s+3} + \\frac{C}{s+1}\n",
    "$$\n",
    "Notice that we don't expand out the numerator on the left hand side.  We will later plug in $s=-3$, so it is convenient to leave this factored.\n",
    "We multiply by the denominator:\n",
    "\n",
    "$$\n",
    "-6 + (s+2)(s+3) = A(s+1) + B(s+3)(s+1) + C(s+3)^2\n",
    "$$\n",
    "\n",
    "Using $s=-3$:\n",
    "\n",
    "$$\n",
    "-6 = -2A \\Rightarrow A=3\n",
    "$$\n",
    "\n",
    "Using $s=-1$:\n",
    "\n",
    "$$\n",
    "-6 +2 = 4C \\Rightarrow C=-1\n",
    "$$\n",
    "\n",
    "Finally another convenient value is $s=0$:\n",
    "\n",
    "$$\n",
    "0 = A + 3B + 9C = 3-9+3B \\Rightarrow B=2\n",
    "$$\n",
    "\n",
    "Thus \n",
    "\n",
    "$$ \\tilde{f}(s) = \\frac{3}{(s+3)^2} + \\frac{2}{s+3} + \\frac{-1}{s+1}$$\n",
    "and\n",
    "\\begin{align*}\n",
    "f(t) &= \\mathcal{L}^{-1}[\\tilde{f}(s)](t)\\\\\n",
    "&= \\mathcal{L}^{-1}\\left[\\frac{3}{(s+3)^2} + \\frac{2}{s+3} + \\frac{-1}{s+1}\\right](t)\\\\\n",
    "&= e^{-3t} \\mathcal{L}^{-1}\\left[\\frac{3}{s^2}\\right](t) + 2 e^{-3t} - e^{-t}\\\\\n",
    "&= 3te^{-3t}+ 2e^{-3t} - e^{-t}\n",
    "\\end{align*}\n",
    "\n",
    "````"
   ]
  },
  {
   "cell_type": "markdown",
   "metadata": {},
   "source": [
    "It is useful to see an example that involves a $t$-shift\n",
    "````{prf:example} $f'(t) + 2f(t) = t H_4(t)$\n",
    "\n",
    "\n",
    "\n",
    "To solve for $f(t)$ when $f'(t) + 2f(t) = t H_4(t)$ with $f(0) = 3$ we follow the same steps, taking the Laplace Transform of both sides.  \n",
    "\n",
    "We have\n",
    "\\begin{align*}\n",
    "\\mathcal{L}[f'(t) + 2f(t)](s) &= \\mathcal{L}[t H_4(t)](s)\\\\\n",
    "s\\tilde{f}(s) - 3 + 2\\tilde{f}(s)  = \\mathcal{L}[t H_4(t)](s)\n",
    "\\end{align*}\n",
    "To do the transform of the discontinuous term, we note that $g(t-4) = t$ if $g(t)=t+4$.  Or we could use the result from the Transform Table (added 2025/03/07) that\n",
    "\n",
    "$$\n",
    "\\mathcal{L}[r(t)H_a(t)](s) = e^{-as} \\mathcal{L}[r(t+a)](s)\n",
    "$$\n",
    "using $r(t) = t$.\n",
    "\n",
    "Either way we end up with $e^{-4s} \\mathcal{L}[t+4](s) = e^{-4s} \\left(\\frac{1}{s^2} + \\frac{4}{s}\\right)$.  Thus we have\n",
    "\\begin{align*}\n",
    "(s+2) \\tilde{f}(s) -3 &=  e^{-4s} \\left(\\frac{1}{s^2} + \\frac{4}{s}\\right)\\\\\n",
    "\\tilde{f}(s) &= \\frac{3}{s+2}  + e^{-4s} \\frac{1+4s}{s^2(s+2)}\n",
    "\\end{align*}\n",
    "\n",
    "We have $\\tilde{f}(s)$ so we are ready to find $f(t)$ by inverting the Laplace Transform.\n",
    "When we invert the transform, we need to handle the part with $e^{-4s}$ and the part without $e^{-4s}$ separately.\n",
    "\\begin{align*}\n",
    "f(t) &= \\mathcal{L}^{-1}[\\tilde{f}(s)](t)\\\\\n",
    "  &= \\mathcal{L}^{-1}\\left[ \\frac{3}{s+2}  + e^{-4s} \\frac{1+4s}{s^2(s+2)}\\right](t)\\\\\n",
    "  &= 3e^{-2t}  + \\mathcal{L}^{-1} \\left[ e^{-4s}\\frac{1+4s}{s^2(s+2)}\\right](t)\\\\\n",
    "  &= 3e^{-2t} + H_4(t) \\mathcal{L}^{-1} \\left[ \\frac{1+4s}{s^2(s+2)}\\right](t-4)\n",
    "\\end{align*}\n",
    "We will use a partial fractions expansion\n",
    "\n",
    "$$\\frac{1+4s}{s^2(s+2)} = \\frac{A}{s^2} + \\frac{B}{s} + \\frac{C}{s+2}\n",
    "$$\n",
    "We get\n",
    "\n",
    "$$\n",
    "1+4s = A(s+2) + B(s)(s+2) + Cs^2\n",
    "$$\n",
    "Taking $s=-2$, we have $4C = -7$ and $C = -7/4$.  Taking $s=0$ gives $2A=1$, so $A=1/2$.  It is convenient to look at the coefficient of $s^2$ to conclude $B+C=0$ so $B=-C = 7/4$.\n",
    "\n",
    "So we finally have\n",
    "\\begin{align*}\n",
    "f(t) &= 3e^{-2t} +  H_4(t) \\mathcal{L}^{-1} \\left[ \\frac{1+4s}{s^2(s+2)}\\right](t-4)\\\\\n",
    "&= 3e^{-2t}  + H_4(t) \\mathcal{L}^{-1} \\left[\\frac{1/2}{s^2} + \\frac{7/4}{s} - \\frac{7/4}{s+2} \\right](t-4)\\\\\n",
    "&= 3e^{-2t} + H_4(t) \\left( \\frac{1}{2}(t-4) + \\frac{7}{4} - \\frac{7}{4}e^{-2(t-4)}\\right)\n",
    "\\end{align*}\n",
    "\n",
    "\n",
    "````"
   ]
  }
 ],
 "metadata": {
  "language_info": {
   "name": "python"
  }
 },
 "nbformat": 4,
 "nbformat_minor": 2
}
