{
 "cells": [
  {
   "cell_type": "markdown",
   "metadata": {},
   "source": [
    "# Inverting the Laplace Transform with Partial Fractions --- higher order denominators"
   ]
  },
  {
   "cell_type": "markdown",
   "metadata": {},
   "source": [
    "## Finding $\\mathcal{L}^{-1}[p(s)/q(s)](t)$ when $q(s)$ is cubic or higher order\n",
    "\n",
    "When $\\tilde{f}(s) = \\frac{p(s)}{q(s)}$ where $q(s)$ is cubic or higher order and $p(s)$ has lower order than $q(s)$, the process is similar to the quadratic case.  We will assume that we know the factored version of $q(s)$ and build up a partial fractions expansion for $p(s)/q(s)$.  \n",
    "\n",
    "We will consider three cases for the factors of $q(s)$:\n",
    "- $(s-a)$ appears as a single unrepeated factor of $q(s)$.  In this case the Partial Fraction expansion will have a term of the form \n",
    "\n",
    "$$\\frac{A}{s-a}$$\n",
    "\n",
    "- $(s-a)^n$ for $n>1$ appears as a factor of $q(s)$.  In this case, the Partial Fraction expansion will have terms of the form\n",
    "\n",
    "$$ \\frac{A_1}{s-a} + \\frac{A_2}{(s-a)^2} + \\cdots + \\frac{A_n}{(s-a)^n}$$\n",
    "\n",
    "- $(s-a)^2 + \\omega^2$ appears as a factor of $q(s)$.  In this case, the Partial Fraction expansion will have a term of the form\n",
    "\n",
    "$$ \\frac{A(s-a) + B\\omega}{(s-a)^2+\\omega^2}$$\n",
    "\n",
    "We are ignoring the possibility that $(s-a)^2 + \\omega^2$ is repeated.  We will address this case in an extension exercise.\n",
    "\n",
    "Once we have built up the full Partial Fraction expansion with terms from all factors of $q(s)$, we use the same approach to find the coefficients.  Then we can invert the transform to find $f(t)$.\n",
    "\n",
    "Notice that in all of the examples, we leave all of the expressions in factored form.  We never expand the product of polynomials.\n"
   ]
  },
  {
   "cell_type": "markdown",
   "metadata": {},
   "source": [
    "\n",
    "````{prf:example} Distinct real roots\n",
    ":label: example:distinct\n",
    "\n",
    "Find $f(t)$ if $\\tilde{f}(s) =  \\frac{7s^2-31s+36}{(s-1)(s-2)(s-3)}$\n",
    "\n",
    "$$\n",
    "\\frac{p(s)}{q(s)} = \\frac{7s^2-31s+36}{(s-1)(s-2)(s-3)}\n",
    "$$\n",
    "\n",
    "We set\n",
    "\\begin{align*}\n",
    "\\frac{p(s)}{q(s)} &= \\frac{A}{s-1} + \\frac{B}{s-2} + \\frac{C}{s-3}\\\\\n",
    "\\Rightarrow \\quad \n",
    "7s^2-31s+36 &= A(s-2)(s-3) + B(s-1)(s-3) + C(s-1)(s-2)\n",
    "\\end{align*}\n",
    "Now we set $s=1$ and get\n",
    "\n",
    "$$\n",
    "12 = A(-1)(-2) \\quad \\Rightarrow \\quad A= 6\n",
    "$$\n",
    "\n",
    "Next we set $s=2$ and get\n",
    "\n",
    "$$\n",
    "2 = B(1)(-1)  \\quad \\Rightarrow \\quad B = -2\n",
    "$$\n",
    "\n",
    "Finally we set $s=3$ and get\n",
    "\n",
    "$$ \n",
    "6= C(2)(1) \\quad \\Rightarrow \\quad C=3\n",
    "$$\n",
    "\n",
    "So \n",
    "\n",
    "$$\n",
    "\\frac{p(s)}{q(s)} = \\frac{6}{s-1} - \\frac{2}{s-2} + \\frac{3}{s-3}\n",
    "$$\n",
    "and\n",
    "\n",
    "$$\n",
    "f(t) = 6e^t - 2 e^{2t} + 3e^{3t}\n",
    "$$\n",
    "\n",
    "````\n"
   ]
  },
  {
   "cell_type": "markdown",
   "metadata": {},
   "source": [
    "### Repeated roots\n",
    "\n",
    "````{prf:example} Repeated Roots\n",
    "\n",
    "Find $f(t)$ if \n",
    "\n",
    "$$\\tilde{f}(s) = \\frac{3s^3 + 10s^2 + 10s +2}{(s+1)^3(s+2)}$$\n",
    "\n",
    "We write out the partial fraction expansion\n",
    "\n",
    "$$\n",
    "\\frac{3s^3 + 10s^2 + 10s +2}{(s+1)^3(s+2)} = \\frac{A}{(s+1)^3} + \\frac{B}{(s+1)^2} + \\frac{C}{s+1} + \\frac{D}{(s+2)} \n",
    "$$\n",
    "Again we multiply by the denominator $p(s)$:\n",
    "\n",
    "$$\n",
    "3s^3 + 10s^2 + 10s +2 = A(s+2) + B(s+1)(s+2) + C(s+1)^2(s+2) + D(s+1)^3\n",
    "$$\n",
    "If we set $s=-1$:\n",
    "\n",
    "$$\n",
    "-1 = A\n",
    "$$\n",
    "\n",
    "If we set $s=-2$:\n",
    "\n",
    "$$\n",
    "-2 = -D \\Rightarrow D=2\n",
    "$$\n",
    "\n",
    "THere are no longer obvious choices for what value of $s$.  We need two more equations to find the remaining two coefficients.  We can find equations by matching coefficients of powers of $s$ or by trying other values of $s$.  It is convenient to try $s=0$ (which is equivalent to matching the coefficient of $s^0$).\n",
    "\\begin{align*}\n",
    "2 &= 2A + 2B + 2C + D\\\\\n",
    "  & = -2 + 2B+2C+2 \\\\\n",
    "  \\Rightarrow B+C&=1\n",
    "\\end{align*}\n",
    "\n",
    "Another convenient option is $s=1$\n",
    "\\begin{align*}\n",
    "25  &= 3A+ 6B + 12C + 8D \\\\\n",
    "    &= -3 + 6B + 12C +16 \\\\\n",
    "\\Rightarrow 6B+12C &= 12\n",
    "\\end{align*}\n",
    "\n",
    "Solving this system gives $B=0$ and $C=1$.  So\n",
    "\n",
    "$$\n",
    "\\tilde{f}(s) = \\frac{-1}{(s+1)^3} + \\frac{1}{s+1} + \\frac{2}{s+2}\n",
    "$$\n",
    "To take the inverse Laplace Transfrom for the term with $(s+1)^3$, we will use the $s$-shift.  We start by breaking up the inverse transfrom into separate pieces:\n",
    "\\begin{align*}\n",
    "f(t) &= \\mathcal{L}^{-1}[\\tilde{f}(s)](t)\\\\\n",
    "     &= \\mathcal{L}^{-1}\\left[\\frac{-1}{(s+1)^3} + \\frac{1}{s+1} + \\frac{2}{s+2}\\right] (t)\\\\\n",
    "     &= \\mathcal{L}^{-1}\\left[\\frac{-1}{(s+1)^3}\\right](t) + e^{-t} + 2 e^{-2t}\n",
    "\\end{align*}\n",
    "Now we apply the $s$-shift:\n",
    "\\begin{align*}\n",
    "f(t) &= -e^{-t} \\mathcal{L}^{-1}\\left[\\frac{1}{s^3}\\right](t)  + e^{-t} + 2 e^{-2t}\\\\\n",
    "     &= -e^{-t}\\frac{1}{2} \\mathcal{L}^{-1}\\left[ \\frac{2}{s^3}\\right](t) + e^{-t} + 2 e^{-2t}\\\\\n",
    "     &= \\frac{-1}{2} e^{-t} t^2 + e^{-t} + 2 e^{-2t}\n",
    "\\end{align*}\n"
   ]
  },
  {
   "cell_type": "markdown",
   "metadata": {},
   "source": [
    "````{prf:example} A quadratic factor that does not factor further\n",
    "\n",
    "Find $f(t)$ if\n",
    "\n",
    "$$\n",
    "\\tilde{f}(s) = \\frac{6s^2-30s+40}{(s-1)\\left((s-3)^2+2^2\\right)}\n",
    "$$\n",
    "\n",
    "The Partial Fractions expansion we use is:\n",
    "\n",
    "$$\n",
    "\\tilde{f}(s) = \\frac{A}{s-1} + \\frac{B(s-3) + 2C}{(s-3)^2 + 2^2}\n",
    "$$\n",
    "Multiplying through by the denominator of $\\tilde{f}(s)$ we get\n",
    "\n",
    "$$\n",
    "6s^2-30s+40 = A\\left((s-3)^2+2^2\\right) + B(s-3)(s-1) + 2C(s-1)\n",
    "$$\n",
    "Choosing $s=1$ gives\n",
    "\n",
    "$$\n",
    "16 = A((-2)^2 + 2^2) + 0B + 0C\n",
    "$$\n",
    "So $A=2$\n",
    "\n",
    "Choosing $s=3$ gives\n",
    "\n",
    "$$\n",
    "4 = 4A + 4C = 8+4C\n",
    "$$\n",
    "and thus $C=-1$.\n",
    "\n",
    "Finally we need one more equation.  We will take $s=0$:\n",
    "\n",
    "$$\n",
    "40 = 13A + 3B -2C = 28 + 3B\n",
    "$$\n",
    "So $B=4$.  Putting it together we have\n",
    "\n",
    "$$\n",
    "\\tilde{f}(s) = \\frac{2}{s-1} + \\frac{4(s-3) - 1(2)}{(s-3)^2+2^2}\n",
    "$$\n",
    "\n",
    "Taking the inverse transform we get\n",
    "\n",
    "$$\n",
    "f(t) = 2e^{t} + 4 e^{3t} \\cos(2t) - e^{3t} \\sin(2t)\n",
    "$$\n",
    "\n",
    "\n",
    "\n",
    "\n",
    "\n"
   ]
  },
  {
   "cell_type": "markdown",
   "metadata": {},
   "source": [
    "## Self-Test\n",
    "\n",
    "1. Write out the correct form of the partial fractions (no need to find the coefficients) for inverting the Laplace Transform of each of the following:\n",
    "````{tab-set}\n",
    "```{tab-item} Q1\n",
    "$$\n",
    "\\tilde{f}(s) = \\frac{2s^2+12s+22}{(s+1)(s+4)(s+5)}\n",
    "$$\n",
    "```\n",
    "```{tab-item} A1 (click tab to see answer)\n",
    "$$\n",
    "\\tilde{f}(s) = \\frac{A}{s+1} + \\frac{B}{s+4} + \\frac{C}{s+5}\n",
    "$$\n",
    "```\n",
    "```` \n",
    "````{tab-set}\n",
    "```{tab-item} Q2\n",
    "$$\n",
    "\\tilde{f}(s) = \\frac{s^2+2s-35}{(s+3)((s+3)^2+4^2)}\n",
    "$$\n",
    "```\n",
    "```{tab-item} A2 (click tab to see answer)\n",
    "$$\n",
    "\\tilde{f}(s) = \\frac{A}{s+3} + \\frac{B(s+3) + 4C}{(s+3)^2+4^2}\n",
    "$$\n",
    "```\n",
    "```` \n",
    "````{tab-set}\n",
    "```{tab-item} Q3\n",
    "$$\n",
    "\\tilde{f}(s) = \\frac{s^4 + 10 s^3 + 38 s^2 + 56 s + 40}{(s+2)^3(s^2+2^2)}\n",
    "$$\n",
    "```\n",
    "```{tab-item} A3 (click tab to see answer)\n",
    "$$\n",
    "\\tilde{f}(s) = \\frac{A}{(s+2)^3} + \\frac{B}{(s+2)^2} + \\frac{C}{(s+2)} + \\frac{Ds+2E}{s^2+2^2}\n",
    "$$\n",
    "```\n",
    "```` \n",
    "2. Find the coefficients of the Partial Fraction Expansion and find $f(t) = \\mathcal{L}^{-1}[f(s)](t)$.\n",
    "````{tab-set}\n",
    "```{tab-item} Q1\n",
    "$$\n",
    "\\tilde{f}(s) = \\frac{2s^2+12s+22}{(s+1)(s+4)(s+5)}\n",
    "$$\n",
    "```\n",
    "```{tab-item} A1 (click tab to see answer)\n",
    "\\begin{align*}\n",
    "\\tilde{f}(s) &= \\frac{1}{s+1} + \\frac{-2}{s+4} + \\frac{3}{s+5}\\\\\n",
    "f(t) &= e^{-t} - 2e^{-4t} + 3e^{-5t}\n",
    "\\end{align*}\n",
    "```\n",
    "```` \n",
    "````{tab-set}\n",
    "```{tab-item} Q2\n",
    "$$\n",
    "\\tilde{f}(s) = \\frac{s^2+2s-35}{(s+3)((s+3)^2+4^2)}\n",
    "$$\n",
    "```\n",
    "```{tab-item} A2 (click tab to see answer)\n",
    "\\begin{align*}\n",
    "\\tilde{f}(s) &= \\frac{-2}{s+3} + \\frac{3(s+3) -1\\cdot 4}{(s+3)^2+4^2}\\\\\n",
    "f(t) &= -2e^{-3t} + 3e^{-3t}\\cos(4t) - e^{-3t}\\sin(4t)\n",
    "\\end{align*}\n",
    "```\n",
    "```` \n",
    "\n",
    "````{tab-set}\n",
    "```{tab-item} Q3\n",
    "$$\n",
    "\\tilde{f}(s) = \\frac{s^4 + 10 s^3 + 38 s^2 + 56 s + 40}{(s+2)^3(s^2+2^2)}\n",
    "$$\n",
    "```\n",
    "```{tab-item} A3 (click tab to see answer)\n",
    "\\begin{align*}\n",
    "\\tilde{f}(s) &= \\frac{2}{(s+2)^3} + \\frac{0}{(s+2)^2} + \\frac{0}{(s+2)} + \\frac{1s+2\\cdot 2}{s^2+2^2}\\\\\n",
    "f(t) &= t^2e^{-2t}+ \\cos(2t) + 2 \\sin(2t) \n",
    "\\end{align*}\n",
    "```\n",
    "```` \n",
    "3. (\\*) The Laplace Transform of $t\\cos(\\omega t)$ and of $t \\sin(\\omega t)$ are\n",
    "\n",
    "\\begin{align*}\n",
    "\\mathcal{L}[t \\cos(\\omega t)](s) &= \\frac{s^2-\\omega^2}{(s^2+\\omega^2)^2}\\\\\n",
    "\\mathcal{L}[t \\sin(\\omega t)](s) &= \\frac{2\\omega s}{(s^2+\\omega^2)^2}\n",
    "\\end{align*}\n",
    "\n",
    "While solving $f''(t) + 9f(t) = \\cos(3t)$ with $f(0)=0$ and $f'(0)=1$ a student discovers that $\\tilde{f}(s) = \\frac{s^2+s+9}{(s^2+3^2)^2}$.  \n",
    "````{tab-set}\n",
    "```{tab-item} Q1\n",
    "What do you think would be a good choice for a Partial Fraction expansion of $\\tilde{f}(s)$?\n",
    "```\n",
    "\n",
    "```{tab-item} A1 (click tab to see answer)\n",
    "More than one reasonable answer exists, but\n",
    "\n",
    "$$\n",
    "\\tilde{f}(s) = \\frac{A(s^2-3^2)}{(s^2+3^2)^2} + \\frac{B (6s)}{(s^2+3^2)^2} + \\frac{Cs}{s^2+3^2} + \\frac{3D}{s^2+3^2}\n",
    "$$\n",
    "is a particularly good choice.\n",
    "```\n",
    "````      \n",
    "````{tab-set}\n",
    "```{tab-item} Q2\n",
    "Using the partial fraction expansion given in Q1, find the coefficients and $f(t)$.  It would help to try matching coefficients of $s$ to get some of the terms.\n",
    "```\n",
    "\n",
    "```{tab-item} A2 (click tab to see answer)\n",
    "Multiplying up by $(s^2+3^2)^2$ we get\n",
    "\n",
    "$$\n",
    "s^2+s+9 = A(s^2-9) + 6Bs + Cs(s^2+9) + 3D(s^2+9)\\\\\n",
    "$$\n",
    "Looking at the coefficients of powers of $s$ yields\n",
    "\\begin{align*}\n",
    "&s^3:\\quad &0 = C\\\\\n",
    "&s^2: \\quad &1= A+ 3D\\\\\n",
    "&s: \\quad &1= 9C+6B\\\\\n",
    "&1: \\quad &9= -9A + 27D\n",
    "\\end{align*}\n",
    "Solving this yields $C=0$,  $B=1/6$,  $D=1/3$, and $A=0$\n",
    "So\n",
    "\n",
    "$$\\tilde{f}(s) =  \\frac{1}{6} \\frac{2\\cdot 3s}{(s^2+3^2)^2} + \\frac{1}{3} \\frac{3}{s^2+3^2} $$\n",
    "\n",
    "and the inverse transform is\n",
    "\n",
    "$$\n",
    "f(t) = \\frac{1}{6} t \\sin(3t) + \\frac{1}{2} \\sin(3t)\n",
    "$$\n",
    "```\n",
    "````      \n",
    "\n"
   ]
  }
 ],
 "metadata": {
  "language_info": {
   "name": "python"
  }
 },
 "nbformat": 4,
 "nbformat_minor": 2
}
